Update ssprove library

coq_ssprove/src/ChoiceEquality.v
@@ -12,123 +12,8 @@ Import RulesStateProb.
 Import RulesStateProb.RSemanticNotation.
 Open Scope rsemantic_scope.
 
-(******************************************************************************)
-(*   This file defines a class ChoiceEquality, which defines an equality      *)
-(* between choice_type and coq types. We also define types both and           *)
-(* both_package, which is stateful code/package and a pure value, combined    *)
-(* with a proof of equality between the two.                                  *)
-(******************************************************************************)
-
-Monomorphic Class ChoiceEquality := {
-    T : Type@{choice.Choice.type.u0} ;
-    ct : choice_type ;
-    ChoiceEq : @eq Type@{choice.Choice.type.u0} (choice.Choice.sort (chElement ct)) T ;
-  }.
-
-Arguments T ChoiceEquality : clear implicits.
-Arguments ct ChoiceEquality : clear implicits.
-Arguments ChoiceEq ChoiceEquality : clear implicits.
-
-Global Coercion T : ChoiceEquality >-> Sortclass.
-Global Coercion ct : ChoiceEquality >-> choice_type.
-
-Definition ct_T {ce : ChoiceEquality} (x : choice.Choice.sort (ct ce)) : T ce :=
-  eq_rect (choice.Choice.sort (chElement (ct ce))) id x (T ce) (ChoiceEq _).
-
-Definition T_ct {ce : ChoiceEquality} (x : T ce) : choice.Choice.sort (ct ce) :=
-  eq_rect_r id x (ChoiceEq _).
-
-Theorem ct_T_id : forall {ce : ChoiceEquality} t, ct_T (T_ct t) = t.
-Proof (fun ce => rew_opp_r id (ChoiceEq ce)).
-
-Theorem T_ct_id : forall {ce : ChoiceEquality} t, T_ct (ct_T t) = t.
-Proof (fun ce => rew_opp_l id (ChoiceEq ce)).
-
-Global Coercion ct_T : choice.Choice.sort >-> T.
-Global Coercion T_ct : T >-> choice.Choice.sort.
-
-
-Lemma ChoiceEquality_ct_EqP : forall ce1 ce2, ce1 = ce2 <-> ct ce1 = ct ce2.
-Proof.
-  split ; intros.
-  - rewrite H.
-    reflexivity.
-  - destruct ce1 as [T1 ct1 CE1].
-    destruct ce2 as [T2 ct2 CE2].
-    cbn in *.
-    subst.
-    reflexivity.
-Qed.
-
-Definition ChoiceEquality_leq (t1 t2 : ChoiceEquality) :=
-    choice_type_leq t1 t2.
-
-Lemma ChoiceEquality_leqP : Ord.axioms ChoiceEquality_leq.
-Proof.
-  unfold ChoiceEquality_leq.
-  destruct choice_type_leqP.
-  split.
-  - intros ?. apply H.
-  - intros ? ? ? ? ?. apply (H0 y x z) ; assumption.
-  - intros ? ? ?.
-    apply ChoiceEquality_ct_EqP.
-    apply H1. assumption.
-  - intros ? ?. apply H2.
-Qed.
-
-Program Instance prod_ChoiceEquality (a b : ChoiceEquality) : ChoiceEquality :=
-  {| T := (@T a) * (@T b) ; ct := (@ct a) × (@ct b); |}.
-Next Obligation.
-  intros.
-  do 2 rewrite ChoiceEq.
-  reflexivity.
-Defined.
-
-Notation "A '× B" := (prod_ChoiceEquality A B) (at level 79, left associativity) : hacspec_scope.
-
-Notation "prod_ce( a , b )" := ((a , b) : prod_ChoiceEquality _ _) : hacspec_scope.
-Notation "prod_ce( a , b , .. , c )" := ((.. ((a , b) : prod_ChoiceEquality _ _) .. , c) : prod_ChoiceEquality _ _) : hacspec_scope.
-
-Program Instance sum_ChoiceEquality (a b : ChoiceEquality) : ChoiceEquality :=
-  {| T := (@T a) + (@T b) ; ct := (@ct a) ∐ (@ct b); |}.
-Next Obligation.
-  intros.
-  do 2 rewrite ChoiceEq.
-  reflexivity.
-Defined.
-
-Notation "A '+ B" := (sum_ChoiceEquality A B) (at level 79, left associativity) : hacspec_scope.
-
-Open Scope hacspec_scope.
-
-Definition fst_CE {A B} (p : A '× B) : A := let '(f,s) := p in f.
-Definition snd_CE {A B} (p : A '× B) : B := let '(f,s) := p in s.
-
-
-Theorem T_ct_id_prod : forall {ceA ceB : ChoiceEquality} a b, @T_ct (prod_ChoiceEquality ceA ceB) (@ct_T ceA a , @ct_T ceB b) = (a , b).
-Proof. now intros [? ? []] [? ? []]. Qed.
-
-Theorem T_ct_prod_propegate : forall {ceA ceB : ChoiceEquality} a b, @T_ct (prod_ChoiceEquality ceA ceB) (a , b) = (T_ct a , T_ct b).
-Proof. now intros [? ? []] [? ? []]. Qed.
-
-Theorem ct_T_prod_propegate : forall {ceA ceB : ChoiceEquality} a b,
-    @ct_T (prod_ChoiceEquality ceA ceB) (a , b) = (ct_T a , ct_T b).
-Proof. now intros [? ? []] [? ? []]. Qed.
-
-Instance nat_ChoiceEquality : ChoiceEquality := {| T := nat ; ct := 'nat ; ChoiceEq := ltac:(reflexivity) |}.
-Instance bool_ChoiceEquality : ChoiceEquality := {| T := bool ; ct := 'bool ; ChoiceEq := ltac:(reflexivity) |}.
-Instance unit_ChoiceEquality : ChoiceEquality := {| T := unit ; ct := 'unit ; ChoiceEq := ltac:(reflexivity) |}.
-
-Definition lift_to_code {ce : ChoiceEquality} {L I} (x : @T ce) : code L I (@ct ce) :=
-  {code ret (T_ct x)}.
-
-Definition evaluate_code {ce : ChoiceEquality} {L I} (x : code L I (@ct ce)) `{match Run sampler x 0 with Some _ => True | _ => False end} : @T ce.
-Proof.
-  destruct (Run sampler x 0).
-  apply (ct_T s).
-  contradiction.
-Defined.
-
+Definition lift_to_code {ce L I} (x : choice.Choice.sort ce) : code L I ce :=
+  {code ret x}.
 
 Definition pre_to_post (P : precond) {A} : postcond A A :=
   fun '(a, h₀) '(b, h₁) => a = b /\ P (h₀ , h₁).
@@ -137,118 +22,111 @@ Definition pre_to_post_ret (P : precond) {A} v : postcond A A :=
 
 Definition true_precond : precond := fun _ => True.
 
-Class both L I (A : ChoiceEquality) :=
+Class both L I (A : choice_type) :=
   {
-    is_pure : A ;
-    is_state : code L I (@ct A) ;
+    is_pure : choice.Choice.sort A ;
+    is_state : code L I A ;
     code_eq_proof_statement :
-    ⊢ ⦃ true_precond ⦄
-          is_state ≈ lift_to_code (L := L) (I := I) (is_pure)
-      ⦃ pre_to_post_ret true_precond (T_ct is_pure) ⦄
+    ⊢ ⦃ true_precond ⦄ is_state ≈ ret (is_pure)
+      ⦃ pre_to_post_ret true_precond (is_pure) ⦄
   }.
 
 Arguments is_pure {_} {_} {_} both.
 Arguments is_state {_} {_} {_} both.
 Arguments code_eq_proof_statement {_} {_} {_} both.
 
-Coercion is_pure : both >-> T.
+Coercion is_pure : both >-> choice.Choice.sort.
 Coercion is_state : both >-> code.
 
-Definition opsigCE := ident * (ChoiceEquality * ChoiceEquality).
-Definition InterfaceCE := list opsigCE.
+(* Lemma helper : *)
+(*   forall (o : opsigCE), *)
+(*     choice.Choice.sort (fst (snd o)) = choice.Choice.sort (src (opsigCE_opsig o)). *)
+(* Proof. now intros [? []]. Qed. *)
 
-Definition opsigCE_opsig := (fun '(i, (s, t)) => (i : ident, (ct s, ct t))).
-Definition IfToCEIf (x : InterfaceCE) : Interface := fset (map opsigCE_opsig x).
+(* Lemma pack_helper : *)
+(*   forall {E : InterfaceCE} {o} (H : In o E), *)
+(*     is_true *)
+(*    (ssrbool.in_mem (opsigCE_opsig o) *)
+(*       (ssrbool.mem (IfToCEIf E))). *)
+(* Proof. *)
+(*   intros. *)
+(*   apply (ssrbool.introT (xseq.InP _ _)). *)
+(*   unfold IfToCEIf. *)
+(*   apply -> (in_remove_fset (T:=opsig_ordType)). *)
+(*   apply in_map. *)
+(*   apply H. *)
+(* Defined. *)
 
-Lemma helper :
-  forall (o : opsigCE),
-    choice.Choice.sort (fst (snd o)) = choice.Choice.sort (src (opsigCE_opsig o)).
-Proof. now intros [? []]. Qed.
+(* Class both_package L I (E : InterfaceCE) := *)
+(*   { *)
+(*     pack_pure : forall o, List.In o E -> fst (snd o) -> snd (snd o) ; *)
+(*     pack_state : package L I (IfToCEIf E) ; *)
+(*     pack_eq_proof_statement : forall i s t (H : In (i,(s,t)) E), forall (v : s), *)
+(*       forall f, (pack pack_state) i = Some *)
+(*     (existT *)
+(*        (fun S0 : choice_type => {T0 : choice_type & choice.Choice.sort S0 -> raw_code T0}) *)
+(*        s (existT (fun T0 : choice_type => choice.Choice.sort s -> raw_code T0) t f)) -> *)
+(*       ⊢ ⦃ true_precond ⦄ *)
+(*           f v *)
+(*           ≈ lift_to_code (L := L) (I := I) (pack_pure (i,(s,t)) H v) *)
+(*       ⦃ pre_to_post_ret true_precond (T_ct (pack_pure (i,(s,t)) H v)) ⦄ *)
+(*   }. *)
 
-Lemma pack_helper :
-  forall {E : InterfaceCE} {o} (H : In o E),
-    is_true
-   (ssrbool.in_mem (opsigCE_opsig o)
-      (ssrbool.mem (IfToCEIf E))).
-Proof.
-  intros.
-  apply (ssrbool.introT (xseq.InP _ _)).
-  unfold IfToCEIf.
-  apply -> (in_remove_fset (T:=opsig_ordType)).
-  apply in_map.
-  apply H.
-Defined.
+(* Arguments pack_pure {_} {_} {_} {_} {_} {_} both_package. *)
+(* Arguments pack_state {_} {_} {_} both_package. *)
 
-Class both_package L I (E : InterfaceCE) :=
-  {
-    pack_pure : forall o, List.In o E -> fst (snd o) -> snd (snd o) ;
-    pack_state : package L I (IfToCEIf E) ;
-    pack_eq_proof_statement : forall i s t (H : In (i,(s,t)) E), forall (v : s),
-      forall f, (pack pack_state) i = Some
-    (existT
-       (fun S0 : choice_type => {T0 : choice_type & choice.Choice.sort S0 -> raw_code T0})
-       s (existT (fun T0 : choice_type => choice.Choice.sort s -> raw_code T0) t f)) ->
-      ⊢ ⦃ true_precond ⦄
-          f v
-          ≈ lift_to_code (L := L) (I := I) (pack_pure (i,(s,t)) H v)
-      ⦃ pre_to_post_ret true_precond (T_ct (pack_pure (i,(s,t)) H v)) ⦄
-  }.
+(* Coercion pack_pure : both_package >-> Funclass. *)
+(* Coercion pack_state : both_package >-> package. *)
 
-Arguments pack_pure {_} {_} {_} {_} {_} {_} both_package.
-Arguments pack_state {_} {_} {_} both_package.
+(* Instance package_both {L I} {x y z} (pkg : both_package L I ((x, (y, z)) :: nil)) (args : y) *)
+(*   : both L I (z). *)
+(* Proof. *)
+(*   destruct pkg as [pure state eq_proof]. *)
+(*   pose (o := (x, (y, z)) : opsigCE). *)
+(*   refine {| is_pure := pure o (List.in_eq _ _) args ; *)
+(*            is_state := {code get_op_default state (opsigCE_opsig o) (args) #with valid_get_op_default _ _ _ state (opsigCE_opsig o) (args) _ (pack_helper (List.in_eq _ _)) } |}. *)
+(*   apply eq_proof. *)
+(*   cbn. *)
+(*   destruct (from_valid_package _ _ _ _ (pack_valid state) (opsigCE_opsig o) (pack_helper (List.in_eq _ _))) as [? []]. *)
+(*   rewrite H. *)
+(*   apply f_equal. *)
+(*   apply f_equal. *)
+(*   apply f_equal. *)
+(*   unfold get_op_default. *)
+(*   cbn. *)
+(*   rewrite H. *)
+(*   destruct choice_type_eqP ; [ | contradiction ]. *)
+(*   destruct choice_type_eqP ; [ | contradiction ]. *)
+(*   rewrite pkg_composition.cast_fun_K. *)
+(*   reflexivity. *)
+(* Defined. *)
 
-Coercion pack_pure : both_package >-> Funclass.
-Coercion pack_state : both_package >-> package.
+(* Program Instance both_package' L I o (bf : T (fst (snd o)) -> both L I (snd (snd o))) *)
+(*   : both_package L I (o :: nil) := *)
+(*   {| *)
+(*     pack_pure := fun o0 H => ltac:((assert (o = o0) by now destruct H) ; subst ; apply bf ; apply X) ; *)
+(*     pack_state := (mkpackage (mkfmap ((fst o, pkg_composition.mkdef _ _ (fun x => bf (ct_T x))) :: nil)) (valid_package1 L I (fst o) (fst (snd o)) (snd (snd o)) (fun x => bf (ct_T x)) (fun x => prog_valid (is_state (bf (ct_T x)))))) ; *)
+(*     pack_eq_proof_statement := _ *)
+(*   |}. *)
+(* Next Obligation. *)
+(*   intros. *)
+(*   destruct H ; [ subst | contradiction ]. *)
+(*   cbn in H0. *)
+(*   rewrite (ssrbool.introT ssrnat.eqnP eq_refl) in H0. *)
+(*   inversion H0. *)
+(*   do 2 apply Eqdep.EqdepTheory.inj_pair2 in H1. *)
+(*   subst. *)
+(*   cbn. *)
+(*   rewrite ct_T_id. *)
+(*   apply bf. *)
+(* Defined. *)
 
-Instance package_both {L I} {x y z} (pkg : both_package L I ((x, (y, z)) :: nil)) (args : y)
-  : both L I (z).
-Proof.
-  destruct pkg as [pure state eq_proof].
-  pose (o := (x, (y, z)) : opsigCE).
-  refine {| is_pure := pure o (List.in_eq _ _) args ;
-           is_state := {code get_op_default state (opsigCE_opsig o) (args) #with valid_get_op_default _ _ _ state (opsigCE_opsig o) (args) _ (pack_helper (List.in_eq _ _)) } |}.
-  apply eq_proof.
-  cbn.
-  destruct (from_valid_package _ _ _ _ (pack_valid state) (opsigCE_opsig o) (pack_helper (List.in_eq _ _))) as [? []].
-  rewrite H.
-  apply f_equal.
-  apply f_equal.
-  apply f_equal.
-  unfold get_op_default.
-  cbn.
-  rewrite H.
-  destruct choice_type_eqP ; [ | contradiction ].
-  destruct choice_type_eqP ; [ | contradiction ].
-  rewrite pkg_composition.cast_fun_K.
-  reflexivity.
-Defined.
-
-Program Instance both_package' L I o (bf : T (fst (snd o)) -> both L I (snd (snd o)))
-  : both_package L I (o :: nil) :=
-  {|
-    pack_pure := fun o0 H => ltac:((assert (o = o0) by now destruct H) ; subst ; apply bf ; apply X) ;
-    pack_state := (mkpackage (mkfmap ((fst o, pkg_composition.mkdef _ _ (fun x => bf (ct_T x))) :: nil)) (valid_package1 L I (fst o) (fst (snd o)) (snd (snd o)) (fun x => bf (ct_T x)) (fun x => prog_valid (is_state (bf (ct_T x)))))) ;
-    pack_eq_proof_statement := _
-  |}.
-Next Obligation.
-  intros.
-  destruct H ; [ subst | contradiction ].
-  cbn in H0.
-  rewrite (ssrbool.introT ssrnat.eqnP eq_refl) in H0.
-  inversion H0.
-  do 2 apply Eqdep.EqdepTheory.inj_pair2 in H1.
-  subst.
-  cbn.
-  rewrite ct_T_id.
-  apply bf.
-Defined.
-
-Program Definition lift_to_both {ce : ChoiceEquality} {L I} (x : @T ce) : both L I ce :=
-  {| is_pure := x ; is_state := @lift_to_code ce L I x |}.
+Program Definition lift_to_both {ce : choice_type} {L I} (x : choice.Choice.sort ce) : both L I ce :=
+  {| is_pure := x ; is_state := {code ret x} |}.
 Next Obligation. intros. apply r_ret. intros. easy. Qed.
 
-Definition both0 (A : ChoiceEquality) := both fset.fset0 [interface] A.
-Definition lift_to_both0 {ce : ChoiceEquality} (x : T ce) : both fset.fset0 [interface] ce := lift_to_both x.
+Definition both0 (A : choice_type) := both fset.fset0 [interface] A.
+Definition lift_to_both0 {ce : choice_type} (x : choice.Choice.sort ce) : both fset.fset0 [interface] ce := lift_to_both x.
 
 Definition lift_code_scope {L1 L2 : {fset Location}} {I1 I2 : {fset opsig}} {A} (c : code L1 I1 A) `{H_loc_incl : List.incl L1 L2} `{H_opsig_incl : List.incl I1 I2} : code L2 I2 A :=
   {code (prog c) #with
@@ -271,7 +149,7 @@ Definition lift_scopeI
 Definition lift_scope0 {L I} {A} (b : both fset.fset0 [interface] A) : both L I A :=
   lift_scope (H_loc_incl := incl_nil_l _) (H_opsig_incl := ltac:(rewrite <- fset0E ; apply incl_nil_l)) b.
 
-Instance both_comparable {A : ChoiceEquality} `{Comparable A} {L I} : Comparable (both L I A) :=
+Instance both_comparable {A : choice_type} `{Comparable (choice.Choice.sort A)} {L I} : Comparable (both L I A) :=
   {|
     ltb x y := ltb (is_pure x) (is_pure y) ;
     leb x y := leb (is_pure x) (is_pure y) ;
@@ -287,14 +165,14 @@ Proof.
   now apply (rpre_weaken_rule _ _ _ H).
 Qed.
 
-Program Instance prod_both {ceA ceB : ChoiceEquality} {L1 L2 : {fset _}} {I1 I2 : {fset _}} (a : both L1 I1 ceA) (b : both L2 I2 ceB) : both (L1 :|: L2) (I1 :|: I2) (ceA '× ceB) :=
+Program Instance prod_both {ceA ceB : choice_type} {L1 L2 : {fset _}} {I1 I2 : {fset _}} (a : both L1 I1 ceA) (b : both L2 I2 ceB) : both (L1 :|: L2) (I1 :|: I2) (ceA × ceB) :=
   {|
     is_pure := (is_pure a , is_pure b) ;
     is_state :=
     {code
        x ← a ;;
        y ← b ;;
-       @ret (prod_ChoiceEquality _ _) (x , y)
+       @ret (chProd _ _) (x , y)
     }
   |}.
 Next Obligation.
@@ -310,10 +188,9 @@ Next Obligation.
 Defined.
 Next Obligation.
   intros.
-  rewrite (T_ct_prod_propegate).
 
   set (r := ret _).
-  pattern (T_ct (is_pure a)) in r.
+  pattern (is_pure a) in r.
   set (g := fun _ => _) in r.
   subst r.
   replace (g a) with (bind (ret a) g) by reflexivity.
@@ -326,7 +203,7 @@ Next Obligation.
   apply forget_precond.
 
   set (r := ret _).
-  pattern (T_ct (is_pure b)) in r.
+  pattern (is_pure b) in r.
   set (g := fun _ => _) in r.
   subst r.
   replace (g b) with (bind (ret b) g) by reflexivity.
@@ -362,14 +239,14 @@ Ltac destruct_choice_type_prod :=
       unfold projT1 in H
   end ;
   repeat match goal with
-  | H : @T (prod_ChoiceEquality _ _) |- _ =>
+  | H : (chProd _ _) |- _ =>
       destruct H
   end ;
   repeat match goal with
   | H : choice.Choice.sort
          (chElement
-            (@ct
-               (prod_ChoiceEquality _ _))) |- _ =>
+            (choice.Choice.sort
+               (chProd _ _))) |- _ =>
       destruct H
   end ;
   repeat match goal with
@@ -599,26 +476,25 @@ Proof.
   reflexivity.
 Qed.
 
-Theorem r_bind_eq : forall {B C : ChoiceEquality} (y : B) (g : choice.Choice.sort B  -> raw_code C), (temp ← ret y ;; g temp) = g y.
+Theorem r_bind_eq : forall {B C : choice_type} (y : choice.Choice.sort B) (g : choice.Choice.sort B  -> raw_code C), (temp ← ret y ;; g temp) = g y.
 Proof. reflexivity. Qed.
 
 Theorem r_bind_trans :
-  forall {B C : ChoiceEquality}
+  forall {B C : choice_type}
      (f : choice.Choice.sort B -> raw_code C)
-    (g : B -> raw_code C) (x : raw_code B) (y : B),
+    (g : choice.Choice.sort B -> raw_code C) (x : raw_code B) (y : choice.Choice.sort B),
   forall (P P_mid : precond) (Q : postcond (choice.Choice.sort C) (choice.Choice.sort C)),
-  forall (H_x_is_y : ⊢ ⦃ P ⦄ x  ≈ ret y ⦃ pre_to_post_ret P_mid (T_ct y) ⦄),
-    (⊢ ⦃ P_mid ⦄ f (T_ct y)  ≈ g y ⦃ Q ⦄) ->
+  forall (H_x_is_y : ⊢ ⦃ P ⦄ x  ≈ ret y ⦃ pre_to_post_ret P_mid (y) ⦄),
+    (⊢ ⦃ P_mid ⦄ f (y)  ≈ g y ⦃ Q ⦄) ->
     ⊢ ⦃ P ⦄ temp ← x ;; f temp ≈ g y ⦃ Q ⦄.
 Proof.
   intros.
-  rewrite <- (ct_T_id y).
-  replace (g (ct_T (T_ct y))) with (temp ← ret (T_ct y) ;; g (ct_T temp)) by reflexivity.
+  replace (g y) with (temp ← ret y ;; g temp) by reflexivity.
 
   pose @r_bind.
-  specialize r with (f₀ := f) (f₁ := fun x => g (ct_T x)).
-  specialize r with (m₀ := x) (m₁ := (ret (T_ct y))).
-  specialize r with (pre := P) (mid := pre_to_post_ret P_mid (T_ct y) ) (post := Q).
+  specialize r with (f₀ := f) (f₁ := fun x => g x).
+  specialize r with (m₀ := x) (m₁ := (ret y)).
+  specialize r with (pre := P) (mid := pre_to_post_ret P_mid y ) (post := Q).
   apply r ; clear r.
 
   - apply H_x_is_y.
@@ -628,38 +504,35 @@ Proof.
     eapply rpre_weaken_rule.
     cbn in H2.
     subst.
-    rewrite ct_T_id.
     apply H.
     intros ? ? []. subst. apply H2.
 Qed.
 
 Theorem r_bind_trans' :
-  forall {B C : ChoiceEquality}
+  forall {B C : choice_type}
      (f : choice.Choice.sort B -> raw_code C)
-    (g : B -> raw_code C) (x : raw_code B) (y : B),
+    (g : choice.Choice.sort B -> raw_code C) (x : raw_code B) (y : choice.Choice.sort B),
   forall (P : precond) (Q : postcond (choice.Choice.sort C) (choice.Choice.sort C)),
-  forall (H_x_is_y : ⊨ repr x ≈ repr (ret (T_ct y)) [{retW (T_ct y, T_ct y)}]),
-    (⊢ ⦃ P ⦄ f (T_ct y)  ≈ g y ⦃ Q ⦄) ->
+  forall (H_x_is_y : ⊨ repr x ≈ repr (ret y) [{retW (y, y)}]),
+    (⊢ ⦃ P ⦄ f ( y)  ≈ g y ⦃ Q ⦄) ->
     ⊢ ⦃ P ⦄ temp ← x ;; f temp ≈ g y ⦃ Q ⦄.
 Proof.
   intros.
 
-  rewrite <- (ct_T_id y).
-
-  replace (g (ct_T (T_ct y))) with (temp ← ret (T_ct y) ;; g (ct_T temp)) by reflexivity.
+  replace (g y) with (temp ← ret y ;; g temp) by reflexivity.
 
   pose @r_bind.
-  specialize r with (f₀ := f) (f₁ := fun x => g (ct_T x)).
-  specialize r with (m₀ := x) (m₁ := (ret (T_ct y))).
-  specialize r with (pre := P) (mid := fun s0 s1 => pre_to_post P s0 s1 /\ fst s1 = T_ct y) (post := Q).
+  specialize r with (f₀ := f) (f₁ := fun x => g x).
+  specialize r with (m₀ := x) (m₁ := (ret y)).
+  specialize r with (pre := P) (mid := fun s0 s1 => pre_to_post P s0 s1 /\ fst s1 = y) (post := Q).
   apply r ; clear r.
 
   - eapply from_sem_jdg.
-    eapply (RulesStateProb.weaken_rule (retW (T_ct y , T_ct y))).
+    eapply (RulesStateProb.weaken_rule (retW (y , y))).
     + apply H_x_is_y.
     + unfold retW.
       intros [] X [? πa1a2] ; cbn in X.
-      specialize (fun x => πa1a2 (x, s) (T_ct y, s0)).
+      specialize (fun x => πa1a2 (x, s) (y, s0)).
 
       unfold proj1_sig.
 
@@ -680,9 +553,6 @@ Proof.
     eapply rpre_weaken_rule.
     2: { intros ? ? []. subst. apply H1. }
     clear H1.
-    cbn in H2.
-    subst.
-    rewrite ct_T_id.
     apply H.
 Qed.
 
@@ -726,9 +596,9 @@ Qed.
 Ltac solve_heap_ignore_remove_set_heap :=
   apply (heap_ignore_remove_set_heap) ; [ apply isolate_mem_section ; apply fset_compute ; apply -> in_remove_fset ; cbn ; repeat (left ; reflexivity || right || reflexivity) | assumption ].
 
-Theorem r_bind_trans_both : forall {B C : ChoiceEquality} {L I} {f : choice.Choice.sort B -> raw_code C} {g : B -> raw_code C} (b : both L I B),
+Theorem r_bind_trans_both : forall {B C : choice_type} {L I} {f : choice.Choice.sort B -> raw_code C} {g : choice.Choice.sort B -> raw_code C} (b : both L I B),
   forall (P : precond) (Q : postcond _ _),
-    (⊢ ⦃ true_precond ⦄ f (T_ct (is_pure b))  ≈ g (is_pure b) ⦃ Q ⦄) ->
+    (⊢ ⦃ true_precond ⦄ f ((is_pure b))  ≈ g (is_pure b) ⦃ Q ⦄) ->
     ⊢ ⦃ P ⦄ temp ← is_state b ;; f temp ≈ g (is_pure b) ⦃ Q ⦄.
 Proof.
   intros.
@@ -858,12 +728,6 @@ Proof.
   apply H.
 Qed.
 
-Ltac remove_T_ct :=
-  progress match goal with
-  | [ |- context[ T_ct ?x ] ] =>
-      replace (T_ct x) with x by reflexivity
-  end.
-
 Ltac pattern_both Hx Hf Hg :=
   (match goal with
    | [ |- context [ prog (@is_state ?L ?I _ ?x) : both _ _ _ ] ] =>
@@ -893,7 +757,6 @@ Ltac match_bind_trans_both :=
   let Hx := fresh in
   let Hf := fresh in
   let Hg := fresh in
-  repeat remove_T_ct
-  ; pattern_both Hx Hf Hg
+  pattern_both Hx Hf Hg
   ; apply (@r_bind_trans_both) with (b := Hx) (f := Hf) (g := Hg)
-  ; intros ; try remove_T_ct ; subst Hf ; subst Hg ; subst Hx ; hnf.
+  ; intros ; subst Hf ; subst Hg ; subst Hx ; hnf.
